\input{preamble}

\usepackage{karnaugh-map}

\begin{document}
\chapter{Задача 3}

\section{Условие}

Доказать в исчислении высказываний (буквы обозначают произвольные
формулы):
\[
    \boxed{
        \lnot((X\band Y)\band \lnot Z) \step (\lnot(\lnot X \to \lnot Y) \lor (Y \to Z))
    }
\] 


\section{Решение}

Нам известно, что
\[
\begin{matrix}
    A\band B = \lnot(A \to \lnot B) && A \lor B = \lnot A \to B
\end{matrix}
\] 
Перепишем формулу:
\[
\lnot\lnot(\lnot(X \to \lnot Y) \to \lnot\lnot Z) \step \lnot\lnot(\lnot X \to \lnot Y) \to (Y \to Z)
\] 


Доказательство:

1) $\lnot\lnot(\lnot(X \to \lnot Y) \to \lnot\lnot Z)$ - Гипотеза

2) $\lnot\lnot(\lnot(X \to \lnot Y) \to \lnot\lnot Z) \to (\lnot(\lnot X \to \lnot Y) \to \lnot\lnot Z)$ -
секвенция 3 при $A := \lnot(X \to \lnot Y) \to \lnot\lnot Z$

3) $\lnot(\lnot X \to \lnot Y) \to \lnot\lnot Z$ - modus ponens, (1) и (2)

4) $\lnot\lnot(\lnot X \to \lnot Y)$ - Гипотеза

5) $\lnot\lnot(\lnot X \to \lnot Y) \to (\lnot X \to \lnot Y)$ - секвенция 3 при $A := 
(\lnot X \to \lnot Y)$

6) $\lnot X \to \lnot Y$ - modus ponens, (4) и (5)

7) $Y$ - Гипотеза

8) $(\lnot X \to \lnot Y) \to (Y \to X)$ - секвенция 6 при $ A:= Y, B := X$

9)  $Y \to X$ - modus pomems, (6) и (8)

10) $X$ - modus ponens, (7) и (9)

11)  $X \to (\lnot \lnot Y\to \lnot(X \to \lnot Y))$ - секвенция 9 при $A:=X, B:=\lnot Y$

12) $\lnot \lnot Y\to \lnot(X \to \lnot Y)$ - modus ponens, (10) и (11)

13)  $Y \to \lnot\lnot Y$ - секвенция 4 при $A:=Y$

14)  $Y \to \lnot(X \to \lnot Y)$ - секвенция 1, (12) и (13) при $A:=Y,B:=\lnot\lnot Y,
C:=\lnot(X \to \lnot Y)$

15) $\lnot(X \to \lnot Y)$ - modus ponens, (7) и (14)

16) $\lnot\lnot Z$ - modus ponens, (3) и (15)

17)  $\lnot\lnot Z \to Z$ - секвенция 3 при $A := Z$

18)  $Z$ - modus ponens, (16) и (17)

\end{document}
